---
title: 我还活着
katex: true
date: 2022-04-25 23:03:17
tags:
cover: /img/2.jpg
---

## 好久没水博客了，别担心，我还活着
写点数学公式
- 证明 $\lim\limits_{n\to \infty}n\left(\dfrac{\pi}{4}-x_{n}\right)=\dfrac{1}{4}$, 其中 
$$
 x_{n} = \sum\limits_{k=1}^{n} \dfrac{n}{n^2+k^2}
$$
- **证明**
更加一般地，我们令 
$$
x_{n} = \dfrac{1}{n}\sum\limits_{k=1}^{n}f\left(\dfrac{k}{n}\right)
$$ 
计算(其中 $f(x)$ 在 (0,1) 连续)
$$
\lim\limits_{n\to \infty} n\left(\int_{0}^{1} f(x)\,\mathrm{d}x-\dfrac{1}{n}\sum\limits_{k=1}^{n}f\left(\dfrac{k}{n}\right)\right)
$$
我们有
$$
\begin{align*}
  &\int_{0}^{1}f(x)\,\mathrm{d}x = \sum\limits_{k=1}^{n}\int_{\frac{k-1}{n}}^{\frac{k}{n}}f(x)\,\mathrm{d}x \\
  &\dfrac{1}{n}\sum\limits_{k=1}^{n}f\left(\dfrac{k}{n}\right) = \sum\limits_{k=1}^{n}\int_{\frac{k-1}{n}}^{\frac{k}{n}}f\left(\dfrac{k}{n}\right)\,\mathrm{d}x
\end{align*}
$$
于是
$$
\begin{align*}
\int_{0}^{1} f(x)\,\mathrm{d}x-\dfrac{1}{n}\sum\limits_{k=1}^{n}f\left(\dfrac{k}{n}\right) &= \sum\limits_{k=1}^{n}\int_{\frac{k-1}{n}}^{\frac{k}{n}}\left[f(x) - f\left(\dfrac{k}{n}\right)\right]\,\mathrm{d}x \\
&= \sum\limits_{k=1}^{n}\int_{\frac{k-1}{n}}^{\frac{k}{n}}f'(\xi_{k})\left(x-\dfrac{k}{n}\right)\,\mathrm{d}x \qquad \xi_{k} \in (x,\frac{k}{n})\\
&= \sum\limits_{k=1}^{n} f'(\eta_{k}) \int_{\frac{k-1}{n}}^{\frac{k}{n}} \left(x-\dfrac{k}{n}\right)\,\mathrm{d}x \qquad \eta_{k} \in (\frac{k-1}{n},\frac{k}{n})\\
&= \sum\limits_{k=1}^{n} f'(\eta_{k})\left(-\dfrac{1}{2n^2}\right)
\end{align*}
$$
再有
$$
\begin{align*}
\fcolorbox{black}{white}{$\color{magenta}\displaystyle\lim\limits_{n\to \infty} n\left(\int_{0}^{1} f(x)\,\mathrm{d}x-\dfrac{1}{n}\sum\limits_{k=1}^{n}f\left(\dfrac{k}{n}\right)\right)$} &= -\dfrac{1}{2n}\sum\limits_{k=1}^{n} f'(\eta_{k}) \\
&\to -\dfrac{1}{2}\int_{0}^{1}f'(x)\,\mathrm{d}x\quad (n\to \infty) \\
&=\fcolorbox{black}{white}{$\color{magenta}\displaystyle\dfrac{1}{2}(f(0)-(1))$}
\end{align*}
$$
本题只需另
$$
f(x) = \dfrac{1}{1+x^2}
$$
即可得到
$$
n\left(\dfrac{\pi}{4}-x_{n}\right) \to \dfrac{1}{4} \quad (n\to \infty)
$$
